theories/Padded.v
@@ -1,0 +1,79 @@
+From Coq Require Export Morphisms Setoid Program.Equality.
+From ITree Require Export ITree ITreeFacts Eq.Rutt.
+From Paco Require Import paco.
+From Coq Require Export Eqdep EqdepFacts.
+
+Require Export HeterogeneousEventRelations.
+
+
+Ltac inj_existT := repeat match goal with | H : existT _ _ _ = _ |- _ => apply inj_pair2 in H end.
+
+Variant paddedF {E R} (F : itree E R -> Prop) : itree' E R -> Prop :=
+  | paddedF_Ret r : paddedF F (RetF r)
+  | paddedF_Tau t : F t -> paddedF F (TauF t)
+  | paddedF_VisTau A e (k : A -> itree E R) :
+    (forall a, F (k a)) -> paddedF F (VisF e (fun a => (Tau (k a ))))
+.
+
+Definition padded_ {E R} F (t : itree E R) := paddedF F (observe t).
+
+Lemma padded_monot {E R} : monotone1 (@padded_ E R).
+Proof.
+  unfold padded_. red. intros. inv IN; econstructor; eauto.
+Qed.
+
+#[global] Hint Resolve padded_monot : paco.
+
+Definition padded {E R} (t : itree E R) : Prop := paco1 padded_ bot1 t.
+
+Lemma padded_Ret E R r : @padded E R (Ret r).
+Proof. pstep. constructor. Qed.
+
+Lemma padded_Tau E R (t : itree E R) : padded t -> padded (Tau t).
+Proof. intros. pstep. constructor. left. auto. Qed.
+
+Lemma padded_VisTau E R A (e : E A) (k : A -> itree E R) :
+  (forall a, padded (k a)) -> padded (Vis e (fun a => Tau (k a))).
+Proof.
+  intros. pstep. red. cbn. constructor. left. apply H.
+Qed.
+
+Lemma padded_Vis_inv E R A (e : E A) (k : A -> itree E R) : 
+  padded (Vis e k ) -> exists k', forall a, k a ≅ Tau (k' a).
+Proof.
+  intro Hek. pinversion Hek. inj_existT. subst. exists k1. reflexivity.
+Qed.
+
+CoFixpoint pad_ {E R} (ot : itree' E R) : itree E R :=
+  match ot with
+  | RetF r => Ret r
+  | TauF t => Tau (pad_ (observe t) )
+  | VisF e k => Vis e (fun a => Tau (pad_ (observe (k a))))
+  end.
+
+Definition pad {E R} (t : itree E R) := pad_ (observe t).
+
+
+Lemma pad_is_padded E R : forall (t : itree E R), padded (pad t).
+Proof.
+  pcofix CIH. pstep. intros. red. unfold pad.
+  destruct (observe t); cbn.
+  - constructor.
+  - constructor. right. eauto.
+  - constructor. right. eauto.
+Qed.
+
+Lemma pad_eutt E R : forall (t : itree E R), t ≈ pad t.
+Proof.
+  pcofix CIH. intros. pstep. red. unfold pad.
+  destruct (observe t); cbn.
+  - constructor. auto.
+  - constructor. right. eauto.
+  - constructor. left. 
+    generalize (k v) as t'.
+    pcofix CIH'. intros. pstep. constructor; auto.
+    destruct (observe t'); cbn.
+    + constructor; auto.
+    + constructor. right. eauto.
+    + constructor. right. eauto.
+Qed.
